some progress in Hoeffding's inequality

NewTry.thy
@@ -2,12 +2,88 @@ theory NewTry
 imports LearningTheory
 begin
 
+
+
+lemma expectation_pair_pmf:
+    "measure_pmf.expectation (pair_pmf p q) f
+      = measure_pmf.expectation p (\<lambda>x. measure_pmf.expectation q (\<lambda>y. f (x, y)))"
+  using nn_integral_pair_pmf'
+  sorry
+
+lemma 
+  fixes f :: "_ \<Rightarrow> _ \<Rightarrow> real"
+  shows expectation_Pi_pmf:
+    "finite A \<Longrightarrow>  measure_pmf.expectation (Pi_pmf A dflt p) (\<lambda>y. prod (\<lambda>x. f x (y x)) A) =
+    (prod (\<lambda>x. measure_pmf.expectation (p x) (\<lambda>v. f x v)) A)"
+proof (induct rule: finite_induct)
+  case empty
+  then show ?case by auto
+next
+  case (insert a A) 
+  have p: "\<And>x y. (\<Prod>xa\<in>A. f xa (if xa = a then x else y xa)) = (\<Prod>xa\<in>A. f xa (y xa))"
+    apply(rule prod.cong) apply simp using insert by auto
+
+  have "measure_pmf.expectation (Pi_pmf (insert a A) dflt p) (\<lambda>y. \<Prod>x\<in>insert a A. f x (y x))
+        = measure_pmf.expectation (p a) (\<lambda>x. f a x * measure_pmf.expectation (Pi_pmf A dflt p) (\<lambda>y. \<Prod>xa\<in>A. f xa (y xa)))"
+    apply(subst Pi_pmf_insert) apply fact apply fact
+    apply simp
+    unfolding expectation_pair_pmf
+    apply(subst prod.insert) apply fact apply fact
+    apply simp unfolding p by simp
+  also have "\<dots> = (\<Prod>x\<in>insert a A. measure_pmf.expectation (p x) (f x))"
+    apply(subst insert(3))
+    apply(subst prod.insert) apply fact apply fact by simp
+  finally  show ?case .
+qed
+
+
+ 
+lemma Pi_pmf_map2:
+  assumes [simp]: "finite A" and "\<And>x. x\<notin>A \<Longrightarrow> f x dflt = dflt'"
+  shows   "Pi_pmf A dflt' (\<lambda>x. map_pmf (f x) (g x)) = map_pmf (\<lambda>h. (\<lambda>x. (f x) (h x))) (Pi_pmf A dflt g)"
+    (is "?lhs = ?rhs")
+proof (rule pmf_eqI)
+  fix h
+  show "pmf ?lhs h = pmf ?rhs h"
+  proof (cases "\<forall>x. x \<notin> A \<longrightarrow> h x = dflt'")
+    case True
+    hence "pmf ?lhs h = (\<Prod>x\<in>A. measure_pmf.prob (g x) (f x -` {h x}))"
+      by (subst pmf_Pi) (auto simp: pmf_map)
+    also have "\<dots> = measure_pmf.prob (Pi_pmf A dflt g) (PiE_dflt A dflt (\<lambda>x. f x -` {h x}))"
+      by (rule measure_Pi_pmf_PiE_dflt [symmetric]) auto
+    also have "PiE_dflt A dflt (\<lambda>x. f x -` {h x}) = ((\<lambda>g x. f x (g x))  -` {h}) \<inter> PiE_dflt A dflt (\<lambda>_. UNIV)"
+      using True by (fastforce simp: assms(2) [symmetric] fun_eq_iff PiE_dflt_def o_def)
+    also have "measure_pmf.prob (Pi_pmf A dflt g) \<dots> = 
+                 measure_pmf.prob (Pi_pmf A dflt g) ((\<lambda>g x. f x (g x)) -` {h})"
+      by (intro pmf_prob_cong) (auto simp: PiE_dflt_def pmf_Pi_outside)
+    also have "\<dots> = pmf ?rhs h" by (simp add: pmf_map)
+    finally show ?thesis .
+  next
+    case False
+    have "pmf ?rhs h = infsetsum (pmf (Pi_pmf A dflt g)) ((\<lambda>g x. f x (g x)) -` {h})"
+      by (simp add: pmf_map measure_pmf_conv_infsetsum)
+    also from False have "\<dots> = infsetsum (\<lambda>_. 0) ((\<lambda>g x. f x (g x)) -` {h})"
+      by (intro infsetsum_cong pmf_Pi_outside) (auto simp: fun_eq_iff o_def assms(2) [symmetric])
+    also have "\<dots> = 0" by simp
+    also from False have "\<dots> = pmf ?lhs h"
+      by (subst pmf_Pi_outside) auto
+    finally show ?thesis ..
+  qed
+qed
+
+
+
+
 definition "mapify f = (\<lambda>x. Some (f x))"
 definition "allmaps C D = {m. dom m = C \<and> ran m \<subseteq> D}"  
 definition "restrictH H C D = {m\<in>(allmaps C D). \<exists>h\<in>H. m \<subseteq>\<^sub>m h}"
 definition "shatters H C D \<longleftrightarrow> allmaps C D = restrictH H C D"
 
 
+
+
+lemma "H\<noteq>{} \<Longrightarrow> card C \<ge> 1 \<Longrightarrow> card D \<ge> 2 \<Longrightarrow> card (restrictH H C D) \<ge> 4"
+  oops
 
 lemma finitemaps: "finite C \<Longrightarrow> finite D \<Longrightarrow> finite (allmaps C D)"
   by (simp add: allmaps_def finite_set_of_finite_maps)
@@ -69,25 +145,23 @@ term measure_pmf.expectation
 
 lemma markov_inequality:
   "measure_pmf.prob D {x. f x > a} \<le> (measure_pmf.expectation D f / a)"
+  using integral_Markov_inequality[where c=a]
+
   sorry
 
-
-lemma fixes f :: "'a \<Rightarrow> real" and C :: real
-  shows brag1: "(\<forall>h\<in>S. f h \<le> C) \<Longrightarrow> Greatest (\<lambda>r. \<exists>x. f x = r) \<le> C"
-  sorry
- 
-lemma fixes f :: "'c \<Rightarrow> real" and C :: real
-  assumes "S \<noteq> {}"   
-  shows brag2: "Greatest (\<lambda>r. \<exists>x\<in>S. f x = r) \<le> C \<Longrightarrow> h\<in>S \<Longrightarrow>  f h \<le> C"
-  sorry
- 
-thm brag2[OF nnH]
- 
+lemma markov_inequality':
+  "
+  integrable (measure_pmf D) f \<Longrightarrow>
+  AE x in measure_pmf D. 0 \<le> f x \<Longrightarrow> a>0 \<Longrightarrow> measure_pmf.prob D {x. f x \<ge> a} \<le> (measure_pmf.expectation D f / a)"
+  using integral_Markov_inequality[where c=a and u=f and M=D, unfolded measure_pmf.emeasure_eq_measure]  
+    sorry
 
 
-thm Max_le_iff
+thm integral_Markov_inequality
+thm integral_Markov_inequality
+thm nn_integral_Markov_inequality
+
    
-    thm subsetlesspmf
 
 lemma A :
   fixes a b :: real
@@ -95,6 +169,7 @@ lemma A :
 
 lemma "abs(PredErr D h - TrainErr S {0..<m} h) \<ge> 0"
   by auto
+
 lemma assumes mgt0: "m>0"
   shows Error_bounded: "abs(PredErr D h - TrainErr S {0..<m::nat} h) \<le> 2"
 proof -
@@ -109,32 +184,45 @@ proof -
   finally show ?thesis .
 qed
 
-
-print_classes
-
-thm cSup_le_iff
-
-lemma fixes f :: "'c \<Rightarrow> real" and C :: real
-  assumes "S \<noteq> {}"   
-      and "\<And>x. f x \<le> 2"
-  shows brag3: "Sup (f ` S) \<le> C \<Longrightarrow> h\<in>S \<Longrightarrow>  f h \<le> C"
-  sorry
-
-
 lemma PredErr_as_expectation:
   "PredErr D h = measure_pmf.expectation (Samples m D) (\<lambda>S. TrainErr S {0..<m} h )"
-  unfolding PredErr_def unfolding TrainErr_def sorry
+  unfolding PredErr_def unfolding TrainErr_def sorry 
 
 
+definition E :: "real pmf \<Rightarrow> real"  where
+  "E M = (\<integral>x. x \<partial> measure_pmf M)"
+term prob_space
+(* abbreviation (in prob_space) "expectation \<equiv> integral\<^sup>L M" 
+    abbreviation (in prob_space) "prob \<equiv> measure M" *)
+lemma "E M = measure_pmf.expectation M id"
+  unfolding E_def         
+  by (metis comp_id fun.map_ident)  
+
+lemma "E (map_pmf f M) = measure_pmf.expectation M f"
+  unfolding E_def       
+  by simp   
+ 
 lemma expectation_mono:
-    "(\<And>x. f x \<le> g x) \<Longrightarrow> measure_pmf.expectation M f \<le> measure_pmf.expectation M g"
-  sorry
+  fixes f::"'c \<Rightarrow> real"
+  shows 
+    "integrable (measure_pmf M) f \<Longrightarrow>
+    integrable (measure_pmf M) u \<Longrightarrow> (\<And>x. x\<in>set_pmf M \<Longrightarrow> f x \<le> u x) \<Longrightarrow> measure_pmf.expectation M f \<le> measure_pmf.expectation M u"
+  apply(rule integral_mono_AE)
+by (auto simp add: AE_measure_pmf_iff)
 
-lemma expectation_const: "measure_pmf.expectation M (\<lambda>_. c) = c"
-    sorry
+
+lemma expectation_const: "measure_pmf.expectation M (\<lambda>_. c::real) = c" 
+  by simp 
+
+lemma E_cong:
+  fixes f::"'a \<Rightarrow> real"
+  shows "(\<forall>x\<in> set_pmf S. (f x) = (u x)) \<Longrightarrow> E (map_pmf f S) = E (map_pmf u S)"
+unfolding E_def integral_map_pmf apply(rule integral_cong_AE)
+apply(simp add: integrable_measure_pmf_finite)+
+by (simp add: AE_measure_pmf_iff)
 
 lemma expectation_cong: "(\<And>m. m\<in>set_pmf M \<Longrightarrow> f m = g m) \<Longrightarrow> measure_pmf.expectation M f = measure_pmf.expectation M g"
-  sorry
+  by (rule integral_cong_AE, simp_all add: AE_measure_pmf_iff) 
 
 
 lemma expectation_Sup_le: "(\<Squnion>h\<in>H. measure_pmf.expectation D (f h))
@@ -145,27 +233,527 @@ lemma expectation_linear:
     "measure_pmf.expectation M (\<lambda>S. measure_pmf.expectation M2 (f S))
         = measure_pmf.expectation M2 (\<lambda>S2. measure_pmf.expectation M (\<lambda>S. f S S2))"
   sorry
+  
+
+(* by auto3 aka Manuel Eberl: *)
+lemma convex_on_exp: 
+  fixes l :: real
+  assumes "l > 0"
+  shows   "convex_on UNIV (\<lambda>x. exp(l*x))"
+  using assms
+  by (intro convex_on_realI[where f' = "\<lambda>x. l * exp (l * x)"]) (auto
+intro!: derivative_eq_intros)
+
+lemma hoeffdings_lemma:
+  fixes a b :: real
+  assumes range: "\<And>i. measure_pmf.prob D {x. a \<le> x \<and> x \<le> b} = 1" 
+  and E0: "measure_pmf.expectation D id = 0" and "l>0" and aleb: "a\<le>b"
+shows  "measure_pmf.expectation D (\<lambda>x. exp (l*x)) \<le> exp ( l^2 *(b-a)^2 / 8)"
+proof -
+  let ?f = "(\<lambda>x. exp (l * x))"
+
+  from range have xbetweenab: "\<And>x. x\<in>set_pmf D \<Longrightarrow> x \<in> {x. a \<le> x \<and> x \<le> b}"
+    sorry
+  have ab: "a<b" and al0: "a<0" and bg0: "0<b" sorry
+
+  (* for integrable side conditions *)
+  thm measure_pmf.integrable_const_bound 
+  thm integrable_measure_pmf_finite
+
+  then  have anb: "a\<noteq>b" by auto    
+  have F: "\<And>x :: real. (1 - (b - x) / (b - a)) = (x-a)/(b-a)"
+  proof -
+    fix x
+    have "1 = (b-a) / (b-a)" using anb by auto
+    have "(1 - (b - x) / (b - a)) = ((b-a) / (b-a) -  (b - x) / (b - a))"
+      using anb by auto
+    also have "\<dots> = ( (b-a)  -  (b - x) ) /  (b - a)" using anb by argo
+    also have "\<dots> = (x-a)/(b-a)" by auto
+    finally show "(1 - (b - x) / (b - a)) = (x-a)/(b-a)" .
+  qed
+
+  have cvon: "convex_on UNIV (\<lambda>x. exp(l*x))" using  convex_on_exp assms(3) by auto
+
+  have *: "\<And>x. a \<le> x \<Longrightarrow> x \<le> b \<Longrightarrow> ?f x \<le> (b - x) / (b - a) * exp (l * a) + (x-a)/(b-a) * exp (l * b)"
+  proof -
+    fix x :: real
+    let ?\<alpha> = "(b-x) / (b-a)"
+    have g: "1 - ?\<alpha> = (x-a) / (b-a)" using F .
+    assume "a \<le> x" "x \<le> b"
+    then have C: "0 \<le> ?\<alpha>" "?\<alpha> \<le> 1" using ab by auto
+  
+    from convex_onD[OF cvon, of _ b a, simplified ] have A:
+      "\<And>t. 0 \<le> t \<Longrightarrow> t \<le> 1 \<Longrightarrow> exp (l * ((1 - t) * b + t * a)) \<le> (1 - t) * exp (l * b) + t * exp (l * a)" .
+
+    have B: "(1 - ?\<alpha>) * b + ?\<alpha> * a = x"
+    proof -
+      have "(1 - ?\<alpha>) * b + ?\<alpha> * a =  ((x-a) / (b-a)) * b + ((b-x) / (b-a)) * a" 
+        unfolding g .. 
+      also have "\<dots> = (x*(b-a)) / (b-a)" by algebra
+      also have "\<dots> = x" using ab by simp
+      finally show ?thesis .
+    qed
+
+    from A[of ?\<alpha>, simplified B, OF C]
+    show "exp (l * x) \<le> (b - x) / (b - a) * exp (l * a) + (x-a)/(b-a) * exp (l * b)"
+      unfolding  g by simp
+  qed
+  
+
+  have "measure_pmf.expectation D ?f \<le> measure_pmf.expectation D (\<lambda>x. (b - x) / (b - a) * exp (l * a) + (x-a)/(b-a) * exp (l * b))"
+    apply(rule expectation_mono) 
+    subgoal sorry
+    subgoal sorry
+    apply(rule *)
+    using xbetweenab by auto
+  also 
+  have "\<dots> = (b - measure_pmf.expectation D id) / (b - a) * exp (l * a) + (measure_pmf.expectation D id-a)/(b-a) * exp (l * b)"
+    (is "?L = ?R")  
+  proof -
+    have "?L = measure_pmf.expectation D (\<lambda>x. (b + (x * -1)) / (b - a) * exp (l * a) + (x + (- a)) / (b - a) * exp (l * b))" by simp
+    also have "\<dots> = measure_pmf.expectation D (\<lambda>x. (b + x * -1) / (b - a) * exp (l * a)) + measure_pmf.expectation D (\<lambda>x. (x + - a) / (b - a) * exp (l * b))"
+      apply(rule Bochner_Integration.integral_add)
+      subgoal sorry
+      subgoal sorry
+      done
+    also have "measure_pmf.expectation D (\<lambda>x. (b + x * -1) / (b - a) * exp (l * a)) = measure_pmf.expectation D (\<lambda>x. (b + x * -1) / (b - a))  * exp (l * a)"
+      by (rule integral_mult_left_zero)
+    also have "measure_pmf.expectation D (\<lambda>x. (b + x * -1) / (b - a)) =  measure_pmf.expectation D (\<lambda>x. (b + x * -1) ) / (b - a)  " 
+      by(rule integral_divide_zero)
+    also have "measure_pmf.expectation D (\<lambda>x. (b + x * -1) ) = measure_pmf.expectation D (\<lambda>_. b) +  measure_pmf.expectation D (\<lambda>x. x * -1 )" 
+      apply(rule Bochner_Integration.integral_add)
+      subgoal sorry
+      subgoal sorry
+      done
+    also have "measure_pmf.expectation D (\<lambda>_. b) = b"
+      using expectation_const by simp
+    also have "measure_pmf.expectation D (\<lambda>x. x * -1) = - measure_pmf.expectation D id"
+      apply(subst integral_mult_left_zero) unfolding id_def by simp
+
+
+    also have "measure_pmf.expectation D (\<lambda>x. (x + - a) / (b - a) * exp (l * b)) = measure_pmf.expectation D (\<lambda>x. (x + - a) / (b - a) )  * exp (l * b)"
+      by (rule integral_mult_left_zero)
+    also have "measure_pmf.expectation D (\<lambda>x. (x + - a) / (b - a) ) =  measure_pmf.expectation D (\<lambda>x. (x + - a) ) / (b - a)  " 
+      by(rule integral_divide_zero)
+    also have "measure_pmf.expectation D (\<lambda>x. (x + - a) ) = measure_pmf.expectation D (\<lambda>x. x) +  measure_pmf.expectation D (\<lambda>_. -a )" 
+      apply(rule Bochner_Integration.integral_add)
+      subgoal sorry
+      subgoal sorry
+      done
+    also have "measure_pmf.expectation D (\<lambda>_. -a) = -a"
+      using expectation_const by simp
+    also have "measure_pmf.expectation D (\<lambda>x. x ) =  measure_pmf.expectation D id"
+      unfolding id_def by simp
+
+    finally
+    show "?L = ?R" by argo
+  qed
+    (*
+    thm integral_add integral_mult_left_zero integral_divide_zero expectation_const
+    thm integral_bij_count_space
+    thm integral_bounded_linear
+    apply(subst integral_bounded_linear[symmetric, where M=D and T="?f" and f=id])
+    subgoal   sorry
+    subgoal   sorry
+    by simp  *)
+  also have "\<dots> = b / (b - a) * exp (l * a) - a/(b-a) * exp (l * b)"
+    by (simp add: E0)
+  finally have 1: "measure_pmf.expectation D ?f \<le> (b / (b - a)) * ?f a - (a/(b-a)) * ?f b" .
+
+  let ?h = "l*(b-a)"
+  let ?p = "-a / (b-a)"
+  let ?L = "\<lambda>h. -h * ?p + ln (1- ?p + ?p * exp h)"
+
+  have 2: "(b / (b - a)) * ?f a - (a/(b-a)) * ?f b = exp (?L ?h)"
+  proof -
+    have nn: "1 - ?p + ?p * exp ?h > 0"
+    proof -
+      have i: "?p \<ge> 0" using ab al0  
+        by (smt divide_nonneg_pos) 
+      have ii: "exp ?h > 1" apply(subst one_less_exp_iff) using assms(3) ab by auto
+      then have "(exp ?h -1) \<ge>0" by simp
+      have "(exp ?h -1) * ?p \<ge> 0" apply(intro mult_nonneg_nonneg) by fact+
+      moreover have "1 - ?p + ?p * exp ?h = 1 + (exp ?h -1) * ?p" by algebra
+      ultimately show ?thesis by argo
+    qed
+    have "exp (?L ?h) = exp (- ?h * ?p) *  exp ( ln (1- ?p + ?p * exp ?h))"
+      using exp_add by fast 
+    also have "exp ( ln (1- ?p + ?p * exp ?h)) = 1- ?p + ?p * exp ?h" using nn by simp
+    finally have "exp (?L ?h) = exp (- ?h * ?p) * (1- ?p + ?p * exp ?h)" . 
+    also have "\<dots> = (exp (- ?h * ?p) - ?p * exp (- ?h * ?p)) + ?p * exp ?h * exp (- ?h * ?p)" by algebra
+    also have "(exp (- ?h * ?p) - ?p * exp (- ?h * ?p)) = (b / (b - a)) * ?f a"
+    proof - 
+      have expand: "exp (l * a) = ((b-a) * exp (l * a)) / (b-a)" using ab by auto
+      have "(exp (- ?h * ?p) - ?p * exp (- ?h * ?p)) = exp (l * a) + a * exp (l * a) / (b - a)" 
+        using ab by simp
+      also have "\<dots> = ((b-a) * exp (l * a) + a * exp (l * a)) / (b - a)"
+        apply(subst expand) by algebra
+      also have "((b-a) * exp (l * a) + a * exp (l * a)) = b *  exp (l * a)" by algebra
+      finally show ?thesis by simp
+    qed
+    also have "?p * exp ?h * exp (- ?h * ?p) = - (a/(b-a)) * ?f b" 
+    proof - 
+      have collapse: "exp (l * (b - a)) * exp (l * a) = exp (l * (b-a) + l *a)" using mult_exp_exp by blast
+      have "?p * exp ?h * exp (- ?h * ?p) = - (a * (exp (l * (b - a)) * exp (l * a)) / (b - a))" 
+        using ab by simp
+      also have "\<dots> = - (a * exp (l * b) / (b - a))"
+        apply(subst collapse) by argo 
+      finally show ?thesis by simp
+    qed
+    finally 
+    show ?thesis by simp
+  qed
+  have 3: "?L ?h \<le> ?h^2 / 8" sorry
+
+  have 4: "?h^2 = l^2 *(b-a)^2" by algebra
+
+  note 1
+  also have "(b / (b - a)) * ?f a - (a/(b-a)) * ?f b = exp (?L ?h)" using 2 by simp
+  also have "\<dots> \<le> exp (?h^2 / 8)" using 3 ..
+  also have "\<dots> \<le> exp ( l^2 *(b-a)^2 / 8)" unfolding 4 ..
+  finally show ?thesis .
+qed
+
+
+lemma braaaaaaa:
+  assumes [simp]: "finite A"
+  shows   "measure_pmf.expectation (Pi_pmf A dflt p) (\<lambda>y. \<Sum>x\<in>A. (Q x) (y x)) =
+             (\<Sum>x\<in>A. measure_pmf.expectation (p x) (Q x))"
+  (* induction over A? *)
+  sorry
 
 term "Pi_pmf {0..<n} undefined (\<lambda>i. D i)"
 term sum              
 term measure_pmf.prob 
 lemma hoeffding_ineq:
   assumes
-      "\<And>i::nat. measure_pmf.expectation (D i) (f i) = \<mu>"
-    and "\<And>i. measure_pmf.prob (D i) {x. a \<le> x \<and> x \<le> b} = 1" 
-  shows "measure_pmf.prob (Pi_pmf {0..<m} dflt D) {\<sigma>. abs(sum  (\<lambda>i. f i (\<sigma> i) - \<mu>) {0..<m} / m) > \<epsilon> }
+      "\<And>i::nat. measure_pmf.expectation (D i) (f i) = \<mu> i"
+    and "\<And>i. measure_pmf.prob (D i) {x. a \<le> x \<and> x \<le> b} = 1"  and "(\<epsilon>::real)>0"
+  shows "measure_pmf.prob (Pi_pmf {0..<m} dflt D) {\<sigma>. abs(sum  (\<lambda>i. f i (\<sigma> i) - \<mu> i) {0..<m} / m) > \<epsilon> }
              \<le> 2 * exp (- 2 * m * \<epsilon>^2 / (b-a)^2 )"
   sorry
 
 
-lemma Lemma_A4:
-  assumes "a>0" "b\<ge>exp 1" "\<And>t. t\<ge>0 \<Longrightarrow> measure_pmf.prob R {x. abs(f x-x')>t}\<le> 2*b*exp(-(t^2)/a^2)"
-  shows "measure_pmf.expectation R (\<lambda>x. abs(f x-x')) \<le> a * (2+ sqrt (ln b))"
-  sorry
 
-lemma expectation_pair_pmf:
-    "measure_pmf.expectation (pair_pmf p q) f
-      = measure_pmf.expectation p (\<lambda>x. measure_pmf.expectation q (\<lambda>y. f (x, y)))"
+
+
+lemma hoeffding_ineq_forreal:
+  assumes
+      "\<And>i::nat. i < m \<Longrightarrow> measure_pmf.expectation (D i) id = \<mu> i"
+    and "\<And>i. i<m \<Longrightarrow> measure_pmf.prob (D i) {x. a \<le> x \<and> x \<le> b} = 1"  and "(\<epsilon>::real)>0"
+  shows "measure_pmf.prob (Pi_pmf {0..<m} dflt D) {\<sigma>. abs(sum  (\<lambda>i. (\<sigma> i) - \<mu> i) {0..<m} / m) > \<epsilon> }
+             \<le> 2 * exp (- 2 * m * \<epsilon>^2 / (b-a)^2 )"
+proof -
+  have ab2: "a<b" sorry
+  have mgt0: "m>0"   sorry
+  {
+    fix D :: "nat \<Rightarrow> real pmf" and a b :: "nat \<Rightarrow> real" and d :: real
+    assume ONE: "\<And>i. i<m \<Longrightarrow> measure_pmf.prob (D i) {x. a i \<le> x \<and> x \<le> b i} = 1"  
+    assume TWO: "\<And>x. x<m \<Longrightarrow> measure_pmf.expectation (D x) (\<lambda>x. id (x / real m)) = 0"
+    assume defd: "\<And>i. i<m \<Longrightarrow> b i - a i = d"
+    assume dgt0: "d>0" 
+    assume ab: "\<And>i. i<m \<Longrightarrow> a i \<le> b i"  
+    assume ab2: "\<And>i. i<m \<Longrightarrow> a i < b i"  
+  thm markov_inequality
+  { fix M and \<epsilon>::real and l :: real
+    assume "l>0"
+    then 
+    have "measure_pmf.prob M {x. x > \<epsilon>} = measure_pmf.prob M {x. exp (l * x) > exp (l * \<epsilon>)}"
+      by simp
+    also have "\<dots> \<le>  measure_pmf.expectation M (\<lambda>x. exp (l * x)) / exp (l * \<epsilon>)"
+      apply(rule markov_inequality) 
+      done
+    finally have "measure_pmf.prob M {x. x > \<epsilon>} \<le> measure_pmf.expectation M (\<lambda>x. exp (l * x)) / exp (l * \<epsilon>)" .
+  } note first = this
+  { 
+    fix   p and Q and l :: real 
+    have "measure_pmf.expectation (Pi_pmf  {0..<m} dflt p) (\<lambda>y. exp (l * (\<Sum>x\<in> {0..<m}. (Q x) (y x) / m) ))
+          = measure_pmf.expectation (Pi_pmf  {0..<m} dflt p) (\<lambda>y. ( \<Prod>x\<in> {0..<m}. exp (l * (Q x) (y x) / m)))"
+      by (auto simp:  sum_distrib_left exp_sum)     
+    also have "\<dots> = (\<Prod>x\<in> {0..<m}. measure_pmf.expectation (p x) (\<lambda>y. ( exp (l * (Q x) y / m))))"
+      by (auto intro: expectation_Pi_pmf)
+    finally have "measure_pmf.expectation (Pi_pmf {0..<m} dflt p) (\<lambda>y. exp (l * (\<Sum>x = 0..<m. Q x (y x) / real m))) =
+                    (\<Prod>x = 0..<m. measure_pmf.expectation (p x) (\<lambda>y. exp (l * Q x y / real m))) ".
+  } note second = this
+  note second' = second[of _ _ "(\<lambda>x y. y)"]
+  note second'_sym = second[of _ _ "(\<lambda>x y. -y)"]
+
+
+  { 
+    fix x :: nat   and l :: real
+    assume xm: "x<m"
+    assume lgt0: "l>0"
+    from mgt0 have p: "\<And>x y. (x / real m \<le> y / real m) \<longleftrightarrow> x \<le> y"  
+      by (smt divide_strict_right_mono of_nat_0_less_iff)      
+    have ahhhh: "\<And>a b. {y. a / real m \<ge>   (y / real m) \<and>  (y / real m) \<ge> b / real m} = {x. a \<ge> x \<and> x \<ge> b}"
+      unfolding p  
+      by simp
+
+    have "measure_pmf.expectation (D x) (\<lambda>y. exp (l * (-y / real m)))
+          = measure_pmf.expectation (map_pmf (\<lambda>y. (-y / real m)) (D x) ) (\<lambda>y. exp (l * y))"
+      by simp 
+    also have "\<dots> \<le>  exp (l\<^sup>2 * (b x / real m - a x / real m)\<^sup>2 / 8)"  
+      apply(rule order.trans)
+       apply(rule hoeffdings_lemma[where a="-b x/m" and b="-a x/m"])
+      subgoal apply(subst measure_map_pmf) 
+        apply simp unfolding ahhhh apply(subst conj_commute)
+        using ONE[OF xm] .
+      subgoal unfolding integral_map_pmf using TWO[OF xm] by simp
+      subgoal using lgt0 .
+      subgoal using mgt0 ab[OF xm] divide_right_mono by force 
+      apply simp
+      done
+    also have "\<dots> =  exp (l\<^sup>2 * (b x  - a x)\<^sup>2 / (8 * (real m)^2))" apply simp
+      unfolding power2_eq_square using ab mgt0 apply (auto simp: algebra_simps)
+      unfolding add_divide_distrib[symmetric] by simp
+    also have "\<dots> =  exp (l\<^sup>2 * d\<^sup>2 / (8 * (real m)^2))"
+      using defd[OF xm] by simp
+    finally have "measure_pmf.expectation (D x) (\<lambda>y. exp (l * (-y / real m))) \<le> exp (l\<^sup>2 * d\<^sup>2 / (8 * (real m)\<^sup>2)) " .
+  } note third_sym = this
+
+  { 
+    fix x :: nat   and l :: real
+    assume xm: "x<m"
+    assume lgt0: "l>0"
+    from mgt0 have p: "\<And>x y. (x / real m \<le> y / real m) \<longleftrightarrow> x \<le> y"  
+      by (smt divide_strict_right_mono of_nat_0_less_iff)      
+    have ahhhh: "\<And>a b. {y. a / real m \<le> y / real m \<and> y / real m \<le> b / real m} = {x. a \<le> x \<and> x \<le> b}"
+      unfolding p  
+      by simp
+
+    have "measure_pmf.expectation (D x) (\<lambda>y. exp (l * (y / real m)))
+          = measure_pmf.expectation (map_pmf (\<lambda>y. (y / real m)) (D x) ) (\<lambda>y. exp (l * y))"
+      by simp 
+    also have "\<dots> \<le>  exp (l\<^sup>2 * (b x / real m - a x / real m)\<^sup>2 / 8)"  
+       apply(rule hoeffdings_lemma[where a="a x/m" and b="b x/m"])
+      subgoal apply(subst measure_map_pmf) 
+        apply simp unfolding ahhhh
+        using ONE[OF xm]  .
+      subgoal unfolding integral_map_pmf using TWO[OF xm] .
+      subgoal using lgt0 .
+      subgoal using mgt0 ab[OF xm] divide_right_mono by force 
+      done
+    also have "\<dots> =  exp (l\<^sup>2 * (b x  - a x)\<^sup>2 / (8 * (real m)^2))" apply simp
+      unfolding power2_eq_square using ab mgt0 apply (auto simp: algebra_simps)
+      unfolding add_divide_distrib[symmetric] by simp
+    also have "\<dots> =  exp (l\<^sup>2 * d\<^sup>2 / (8 * (real m)^2))"
+      using defd[OF xm] by simp
+    finally have "measure_pmf.expectation (D x) (\<lambda>y. exp (l * (y / real m))) \<le> exp (l\<^sup>2 * d\<^sup>2 / (8 * (real m)\<^sup>2)) " .
+  } note third = this
+
+  note first second
+  {
+    fix l::real
+    assume lgt0: "l>0"
+
+    have "(\<Prod>x = 0..<m. measure_pmf.expectation (D x) (\<lambda>y. exp (l *  y / real m)))
+            = (\<Prod>x = 0..<m. measure_pmf.expectation (D x) (\<lambda>y. exp (l * (y / real m))))" by simp
+    also have "\<dots> \<le> (\<Prod>x = 0..<m. exp (l\<^sup>2 * d\<^sup>2 / (8 * (real m)\<^sup>2)))"
+      apply(rule prod_mono)
+      apply rule
+      subgoal for x apply(rule Bochner_Integration.integral_nonneg) by simp  
+      subgoal apply(rule third) using lgt0 by simp_all
+      done
+    finally have "(\<Prod>x = 0..<m. measure_pmf.expectation (D x) (\<lambda>y. exp (l *   y / real m)))
+           \<le> (\<Prod>x = 0..<m. exp (l\<^sup>2 * d\<^sup>2 / (8 * (real m)\<^sup>2))) " .
+  } note third' = this 
+  {
+    fix l::real
+    assume lgt0: "l>0"
+
+    have "(\<Prod>x = 0..<m. measure_pmf.expectation (D x) (\<lambda>y. exp (l *  -y / real m)))
+            = (\<Prod>x = 0..<m. measure_pmf.expectation (D x) (\<lambda>y. exp (l * (-y / real m))))" by simp
+    also have "\<dots> \<le> (\<Prod>x = 0..<m. exp (l\<^sup>2 * d\<^sup>2 / (8 * (real m)\<^sup>2)))"
+      apply(rule prod_mono)
+      apply rule
+      subgoal for x apply(rule Bochner_Integration.integral_nonneg) by simp  
+      subgoal apply(rule third_sym) using lgt0 by simp_all
+      done
+    finally have "(\<Prod>x = 0..<m. measure_pmf.expectation (D x) (\<lambda>y. exp (l *   -y / real m)))
+           \<le> (\<Prod>x = 0..<m. exp (l\<^sup>2 * d\<^sup>2 / (8 * (real m)\<^sup>2))) " .
+  } note third'_sym = this 
+
+  note first second third'
+
+  let ?avg = "(\<lambda>y. (\<Sum>x = 0..<m. y x / real m))"
+  { fix l :: real and \<epsilon> :: real
+    assume lgt0: "0<l" 
+    have blaub: "(real m * (l\<^sup>2 * d\<^sup>2 / (8 * (real m)\<^sup>2))) - l * \<epsilon> = ( (l\<^sup>2 * d\<^sup>2 / (8 * (real m)))) - l * \<epsilon>" 
+      using mgt0 lgt0  unfolding power2_eq_square 
+      by(auto) 
+
+    from first[OF lgt0, of "map_pmf ?avg (Pi_pmf {0..<m} dflt D)" \<epsilon>]
+    have "measure_pmf.prob (map_pmf ?avg (Pi_pmf {0..<m} dflt D)) {x. \<epsilon> < x}
+          \<le> measure_pmf.expectation (map_pmf ?avg (Pi_pmf {0..<m} dflt D)) (\<lambda>x. exp (l * x)) / exp (l * \<epsilon>)" .
+    also have "\<dots> = measure_pmf.expectation (Pi_pmf {0..<m} dflt D) (\<lambda>x. exp (l * ?avg x)) / exp (l * \<epsilon>)" 
+      by simp
+    also have "\<dots> = (\<Prod>x = 0..<m. measure_pmf.expectation (D x) (\<lambda>y. exp (l * y / real m))) / exp (l * \<epsilon>)" 
+      apply(subst second'[of D l]) ..
+    also have "\<dots> \<le> (\<Prod>x = 0..<m. exp (l\<^sup>2 * d\<^sup>2 / (8 * (real m)\<^sup>2))) / exp (l * \<epsilon>)" 
+       apply(rule divide_right_mono) apply(rule third') subgoal by fact
+      subgoal by simp
+      done
+    also
+    have "\<dots> \<le> exp (l\<^sup>2 * d\<^sup>2 / (8 * real m) - l * \<epsilon>)"
+      apply simp apply(subst exp_of_nat_mult[symmetric])
+      apply(subst exp_diff[symmetric])
+      apply(subst blaub) ..
+    finally have "measure_pmf.prob (map_pmf ?avg (Pi_pmf {0..<m} dflt D)) {x. \<epsilon> < x}
+                   \<le> exp (l\<^sup>2 * d\<^sup>2 / (8 * real m) - l * \<epsilon>) " .
+  } note oneside = this
+
+
+  let ?mavg = "(\<lambda>y. -(\<Sum>x = 0..<m. y x / real m))"
+  { fix l :: real and \<epsilon> :: real
+    assume lgt0: "0<l" 
+    have blaub: "(real m * (l\<^sup>2 * d\<^sup>2 / (8 * (real m)\<^sup>2))) - l * \<epsilon> = ( (l\<^sup>2 * d\<^sup>2 / (8 * (real m)))) - l * \<epsilon>" 
+      using mgt0 lgt0  unfolding power2_eq_square 
+      by(auto) 
+
+    have ppa: "\<And>x. ?mavg x = (\<Sum>xa = 0..<m. - x xa / real m)"
+      using mgt0 unfolding sum_negf[symmetric] by simp
+    from first[OF lgt0, of "map_pmf ?mavg (Pi_pmf {0..<m} dflt D)" \<epsilon>]
+    have "measure_pmf.prob (map_pmf ?mavg (Pi_pmf {0..<m} dflt D)) {x. \<epsilon> < x}
+          \<le> measure_pmf.expectation (map_pmf ?mavg (Pi_pmf {0..<m} dflt D)) (\<lambda>x. exp (l * x)) / exp (l * \<epsilon>)" .
+    also have "\<dots> = measure_pmf.expectation (Pi_pmf {0..<m} dflt D) (\<lambda>x. exp (l * ?mavg x)) / exp (l * \<epsilon>)" 
+      by simp
+    also have "\<dots> = measure_pmf.expectation (Pi_pmf {0..<m} dflt D) (\<lambda>x. exp (l * (\<Sum>xa = 0..<m. - x xa / real m))) / exp (l * \<epsilon>)" 
+      unfolding ppa by simp
+    also have "\<dots> = (\<Prod>x = 0..<m. measure_pmf.expectation (D x) (\<lambda>y. exp (l * -y / real m))) / exp (l * \<epsilon>)"  
+      apply(subst second'_sym[of D l]) ..
+    also have "\<dots> \<le> (\<Prod>x = 0..<m. exp (l\<^sup>2 * d\<^sup>2 / (8 * (real m)\<^sup>2))) / exp (l * \<epsilon>)" 
+       apply(rule divide_right_mono) apply(rule third'_sym) subgoal by fact
+      subgoal by simp
+      done
+    also
+    have "\<dots> \<le> exp (l\<^sup>2 * d\<^sup>2 / (8 * real m) - l * \<epsilon>)"
+      apply simp apply(subst exp_of_nat_mult[symmetric])
+      apply(subst exp_diff[symmetric])
+      apply(subst blaub) ..
+    finally have "measure_pmf.prob (map_pmf ?mavg (Pi_pmf {0..<m} dflt D)) {x. \<epsilon> < x}
+                   \<le> exp (l\<^sup>2 * d\<^sup>2 / (8 * real m) - l * \<epsilon>) " .
+  } note otherside = this
+
+  have aaah: "(4 * real m * \<epsilon> / d\<^sup>2)\<^sup>2 * d\<^sup>2 / (8 * real m) - 4 * real m * \<epsilon> * \<epsilon> / d\<^sup>2
+        = - 2 * m * \<epsilon>^2 / d^2"
+  proof -
+    have p: "(4 * real m * \<epsilon> / d\<^sup>2)\<^sup>2 * d\<^sup>2 / (8 * real m)
+         = (4 * real m * \<epsilon>)^2 * d^2 / (8 * real m*(d^2)*(d^2))"
+      unfolding power2_eq_square using ab  by(auto simp: algebra_simps) 
+    also have "\<dots> = (4 * real m * \<epsilon>)^2  / (8 * real m*(d^2))"
+      using ab by simp
+    finally have 1: "(4 * real m * \<epsilon> / d\<^sup>2)\<^sup>2 * d\<^sup>2 / (8 * real m) = (4 * real m * \<epsilon>)\<^sup>2 / (8 * real m * d\<^sup>2) " .
+
+    have 2: "4 * real m * \<epsilon> * \<epsilon> / d\<^sup>2 = 4 * real m * \<epsilon> * \<epsilon> * 8 * real m / (8 * real m * d\<^sup>2)"
+      using mgt0 by auto
+
+    have "(4 * real m * \<epsilon> / d\<^sup>2)\<^sup>2 * d\<^sup>2 / (8 * real m) - 4 * real m * \<epsilon> * \<epsilon> / d\<^sup>2
+        = (4 * real m * \<epsilon>)\<^sup>2 / (8 * real m * d\<^sup>2) - 4 * real m * \<epsilon> * \<epsilon> * 8 * real m / (8 * real m * d\<^sup>2)"
+      unfolding 1 2 ..
+    also have "\<dots> = ( (4 * real m * \<epsilon>)*(4 * real m * \<epsilon>)  - 4 * real m * \<epsilon> * \<epsilon> * 8 * real m) / (8 * real m * d\<^sup>2)"
+      by algebra
+    also have "\<dots> = ( (8 * real m )*(2 * real m * \<epsilon>* \<epsilon>)  - (8 * real m )*  \<epsilon> * \<epsilon> * 4 * real m) / (8 * real m * d\<^sup>2)"
+      by algebra
+    also have "\<dots> = ( (2 * real m * \<epsilon>* \<epsilon>)  -   \<epsilon> * \<epsilon> * 4 * real m) / (  d\<^sup>2)"
+      using mgt0 by auto
+    
+    also have "\<dots> = - 2 * m * \<epsilon>^2 / d^2" unfolding power2_eq_square using ab mgt0 by (auto simp: algebra_simps) 
+    finally show ?thesis .
+  qed
+  have br: "0 < real (4 * m) * \<epsilon> / d\<^sup>2" apply(rule divide_pos_pos)
+    unfolding power2_eq_square using dgt0  assms(3) mgt0  by auto
+  from oneside[of "4*m*\<epsilon>/d^2" \<epsilon>, OF br] have 
+      "measure_pmf.prob (map_pmf ?avg (Pi_pmf {0..<m} dflt D)) {x. \<epsilon> < x}
+          \<le> exp ((real (4 * m) * \<epsilon> / d\<^sup>2)\<^sup>2 * d\<^sup>2 / (8 * real m) - real (4 * m) * \<epsilon> / d\<^sup>2 * \<epsilon>)"
+    .
+  also have "\<dots> = exp (- 2 *  m * \<epsilon>\<^sup>2 / d\<^sup>2)"
+    apply auto unfolding aaah  by simp
+  finally have
+      "measure_pmf.prob (map_pmf ?avg (Pi_pmf {0..<m} dflt D)) {x. \<epsilon> < x}
+                   \<le> exp (- 2 * m * \<epsilon>\<^sup>2 / d\<^sup>2)" .
+  then have ONESIDE: "measure_pmf.prob (Pi_pmf {0..<m} dflt D) {x. \<epsilon> < ?avg x}
+                   \<le> exp (- 2 * m * \<epsilon>\<^sup>2 / d\<^sup>2)" by simp
+
+  have gr: "\<And>f. {y. \<epsilon> < - f y} = {x. f x < - \<epsilon>}" by auto
+  from otherside[of "4*m*\<epsilon>/d^2" \<epsilon>, OF br] have 
+      "measure_pmf.prob (map_pmf ?mavg (Pi_pmf {0..<m} dflt D)) {x. \<epsilon> < x}
+          \<le> exp ((real (4 * m) * \<epsilon> / d\<^sup>2)\<^sup>2 * d\<^sup>2 / (8 * real m) - real (4 * m) * \<epsilon> / d\<^sup>2 * \<epsilon>)"
+    .
+  also have "\<dots> = exp (- 2 *  m * \<epsilon>\<^sup>2 / d\<^sup>2)"
+    apply auto unfolding aaah  by simp
+  finally  
+  have 
+      "measure_pmf.prob (map_pmf ?mavg (Pi_pmf {0..<m} dflt D)) {x. \<epsilon> < x}
+                   \<le> exp (- 2 * m * \<epsilon>\<^sup>2 / d\<^sup>2)" .
+  then have OTHERSIDE: "measure_pmf.prob (Pi_pmf {0..<m} dflt D) {x. -\<epsilon> > ?avg x}
+                   \<le> exp (- 2 * m * \<epsilon>\<^sup>2 / d\<^sup>2)" apply simp
+    unfolding gr . 
+
+  have p: "\<And>f. {\<sigma>. \<epsilon> < \<bar>f \<sigma>\<bar>} \<subseteq> {x. \<epsilon> < f x} \<union> {x. -\<epsilon> > f x}"
+    by auto  
+  have a: "\<And>\<sigma>. (\<Sum>i = 0..<m. (\<sigma> i)) / real m = (\<Sum>i = 0..<m. (\<sigma> i) / real m)" 
+    using mgt0 sum_divide_distrib by blast  
+  have blub: "{\<sigma>. \<epsilon> < \<bar>(\<Sum>i = 0..<m. (\<sigma> i)) / real m\<bar>} \<subseteq> {x. \<epsilon> < ?avg x} \<union> {x. -\<epsilon> > ?avg x}"
+    unfolding a apply(rule p) .
+
+
+  have "measure_pmf.prob (Pi_pmf {0..<m} dflt D) {\<sigma>. \<epsilon> < \<bar>(\<Sum>i = 0..<m. (\<sigma> i)) / real m\<bar>}
+           \<le> 2 * exp (- 2 * real m * \<epsilon>\<^sup>2 / d\<^sup>2)"
+    apply(rule order.trans)
+     apply(rule subsetlesspmf) apply(rule blub)
+    apply(rule order.trans)
+     apply(rule measure_pmf.finite_measure_subadditive)
+    subgoal by simp
+    subgoal by simp
+    apply(rule order.trans)
+     apply(rule add_mono)
+      apply(rule  ONESIDE)
+     apply(rule OTHERSIDE)
+    by simp 
+} note aname = this
+
+  let ?\<mu> = "\<lambda>i. measure_pmf.expectation (D i) id"
+  thm aname[of "\<lambda>i. map_pmf (\<lambda>x. x - measure_pmf.expectation (D i) id) (D i)"
+            "\<lambda>x. a-?\<mu> x" "\<lambda>x. b-?\<mu> x" "b-a", simplified ] Pi_pmf_map
+
+  have "measure_pmf.prob (Pi_pmf {0..<m} dflt D) {\<sigma>. \<epsilon> < \<bar>(\<Sum>i = 0..<m.  (\<sigma> i) - \<mu> i) / real m\<bar>}
+    = measure_pmf.prob (map_pmf (\<lambda>\<sigma>. (\<lambda>i. if i<m then \<sigma> i - \<mu> i else dflt)) (Pi_pmf {0..<m} dflt D))
+          {\<sigma>. \<epsilon> < \<bar>(\<Sum>i = 0..<m. \<sigma> i) / real m\<bar>}" by simp
+    also have "\<dots>  = measure_pmf.prob (Pi_pmf {0..<m} dflt
+          (\<lambda>i. map_pmf (\<lambda>v. if i<m then v - \<mu> i else dflt)  (D i))
+        ) {\<sigma>. \<epsilon> < \<bar>(\<Sum>i = 0..<m. \<sigma> i) / real m\<bar>}"
+      apply(subst Pi_pmf_map2[where dflt =dflt]) by simp_all 
+  also have "\<dots> \<le> 2 * exp (- 2 * real m * \<epsilon>\<^sup>2 / (b - a)\<^sup>2)" 
+     apply(rule aname[of _ "\<lambda>x.   a-\<mu> x" "\<lambda>x.   b-\<mu> x" "b-a"]) 
+    subgoal apply simp using assms(2) .
+    subgoal for i apply simp
+    proof -
+      assume *: " i < m"
+      have "measure_pmf.expectation (D i) (\<lambda>x. x - \<mu> i) = measure_pmf.expectation (D i) (\<lambda>x. x + (- \<mu> i))" by simp
+      also have "\<dots> = measure_pmf.expectation (D i) (\<lambda>x. x) + measure_pmf.expectation (D i) (\<lambda>x. (- \<mu> i))"
+        apply(rule Bochner_Integration.integral_add) apply auto sorry
+      also have "measure_pmf.expectation (D i) (\<lambda>x. x) = \<mu> i"  using assms(1)[OF *] unfolding id_def  by simp
+      also have "measure_pmf.expectation (D i) (\<lambda>x. (- \<mu> i))  = - \<mu> i"
+        by simp
+      finally show "measure_pmf.expectation (D i) (\<lambda>x. x - \<mu> i) = 0 " by simp
+    qed
+    subgoal by simp
+    subgoal using ab2 by simp
+    subgoal using ab2 by simp
+    subgoal using ab2 by simp
+    done
+  finally show "measure_pmf.prob (Pi_pmf {0..<m} dflt D) {\<sigma>. \<epsilon> < \<bar>(\<Sum>i = 0..<m.   (\<sigma> i) - \<mu> i) / real m\<bar>}
+           \<le> 2 * exp (- 2 * real m * \<epsilon>\<^sup>2 / (b - a)\<^sup>2)" .
+qed
+ 
+
+
+
+
+
+lemma Lemma_A4:
+  assumes "a>0" "b\<ge>exp 1" "\<And>t. t>0 \<Longrightarrow> measure_pmf.prob R {x. abs(f x-x')>t}\<le> 2*b*exp(-(t^2)/a^2)"
+  shows "measure_pmf.expectation R (\<lambda>x. abs(f x-x')) \<le> a * (2+ sqrt (ln b))"
   sorry
 
 
@@ -382,6 +970,9 @@ lemma fixes f :: "'e \<Rightarrow> 'd \<Rightarrow> real"
   by (metis (no_types, lifting) Max_in finite_imageI imageE image_is_empty mem_Collect_eq)  
 
 
+lemma set_pmf_Samples: "\<And>S i. S \<in> set_pmf (Samples m D) \<Longrightarrow> i < m \<Longrightarrow> S i \<in> set_pmf D"
+  sorry
+ 
 
 lemma assumes "set_pmf D \<subseteq> (X\<times>Y)"
       and delta_nn: "\<delta>\<in>{x.0<x\<and>x<1}"
@@ -391,9 +982,12 @@ lemma assumes "set_pmf D \<subseteq> (X\<times>Y)"
 proof -
   have bnd_gt0: "?bnd > 0"   sorry
   have m_gt0: "m>0" sorry
-
-
   have finiteY: "finite Y" sorry (* hmm, not so sure here! *)
+
+  
+  have samples_domain: "\<And>S i. S \<in> set_pmf (Samples m D) \<Longrightarrow> i < m \<Longrightarrow> S i \<in> (X\<times>Y)"
+    using assms(1)  set_pmf_Samples by blast
+
 
   thm measure_pmf.jensens_inequality[where q=abs]
   thm measure_pmf.jensens_inequality[where q=A]
@@ -415,18 +1009,23 @@ proof -
              @{term "h\<in>(restrictH H_map ?C Y)"}. Therefore,\<close>
 
     have pp: "\<And>S. card {fst (S i)|i. i\<in>{0..<m}} \<le> m"
-      apply auto sorry
+      apply(rule order.trans)
+       apply(rule surj_card_le[where A="{0..<m}"])   by auto
+
     have "card ?C \<le> card {fst (S i)|i. i\<in>{0..<m}} + card {fst (S' i)|i. i\<in>{0..<m}}"
       by (rule card_Un_le)
     also have "\<dots> \<le> 2*m"
       using pp[of S] pp[of S'] by simp
-    finally have cardC: "card ?C \<le> 2 * m" .
+    finally have cardC: "card ?C \<le> 2 * m" . 
 
+    have C_nonempty: "?C \<noteq> {}" using m_gt0 by auto
     
     have finite_restrC: "finite (restrictH H_map ?C Y)"
       apply(rule finiteres) apply simp using finiteY by simp
-  
-    have CX: "?C \<subseteq> X" sorry
+
+    assume "S \<in> set_pmf (Samples m D)" "S' \<in> set_pmf (Samples m D)"
+    with samples_domain have CX: "?C \<subseteq> X"  
+      by fastforce  
     have *: "card (restrictH H_map ?C Y) \<le> growth (card ?C)"
       unfolding growth_def
       apply(rule Max_ge)
@@ -436,7 +1035,8 @@ proof -
     have C_bd_growth: "card (restrictH H_map ?C Y) \<le> growth (2*m)"
       apply(rule order.trans)
       apply(rule *) apply(rule growth_mono)  apply(rule cardC) done
-    have C_gt0: "card ?C > 0" apply simp sorry
+    have C_gt0: "card ?C > 0" using m_gt0 by(auto simp add: card_gt_0_iff)
+    have finite_C: "finite ?C" using cardC C_nonempty m_gt0 by auto
     term "MAXIMUM"
     term "restrictH H_map ?C Y"
     have "
@@ -477,6 +1077,10 @@ proof -
 
       show ?thesis 
         apply(rule expectation_mono)
+        subgoal unfolding Samples1_def apply(rule measure_pmf.integrable_const_bound[where B=1])
+          apply auto
+          sorry
+        subgoal unfolding Samples1_def apply auto sorry
         subgoal for \<sigma>
       apply(rule ord_le_eq_trans[OF _ cSup_eq_Max])
       subgoal 
@@ -501,27 +1105,50 @@ proof -
     done
   qed 
   also
-      let ?bla = "\<lambda>\<sigma> h. (sum (\<lambda>i. \<sigma> i * ( (case (S' i) of (x,y) \<Rightarrow> if h x \<noteq> Some y then 1::real else 0)  
-                         -  (case (S i) of (x,y) \<Rightarrow> if h x \<noteq> Some y then 1::real else 0))) {0..<m})    / m "
+  let ?bl = "(\<lambda>v h i. v * ( (case (S' i) of (x,y) \<Rightarrow> if h x \<noteq> Some y then 1::real else 0)  
+                         -  (case (S i) of (x,y) \<Rightarrow> if h x \<noteq> Some y then 1::real else 0)))"
+  let ?blub = "(\<lambda>\<sigma> h i.?bl (\<sigma> i) h i )"
+      let ?bla = "\<lambda>\<sigma> h. (sum (?blub \<sigma> h) {0..<m})    / m "
     { 
       term measure_pmf.prob
-      fix h :: "'a \<Rightarrow> 'b option"   
-      { fix \<rho> D and f :: "nat \<Rightarrow> real \<Rightarrow> real"
-          have "(\<And>i::nat. measure_pmf.expectation (D i) (f i) = 0) \<Longrightarrow>
-  (\<And>i. measure_pmf.prob (D i) {x. -1 \<le> x \<and> x \<le> 1} = 1) \<Longrightarrow>
-  measure_pmf.prob (Pi_pmf {0..<m} 1 D) {\<sigma>. \<rho> < \<bar>(\<Sum>i = 0..<m. f i (\<sigma> i) ) / real m\<bar>}
-  \<le> 2 * exp (-  real m * \<rho>\<^sup>2 / 2 )"
-        using hoeffding_ineq[where \<epsilon>=\<rho> and m=m and a="-1" and b=1 and \<mu>=0 and f=f, simplified] by simp  
-    } note bla = this
-      have "\<And>\<rho>::real. measure_pmf.prob (Samples1 m (pmf_of_set {-1,1::real})) {\<sigma>. \<bar>?bla \<sigma> h\<bar> > \<rho> }
-                    \<le> 2 * exp (-  real m  * \<rho>^2 / 2)"
-        subgoal for \<rho> unfolding Samples1_def
-          apply(rule bla) 
-          subgoal by(simp add: integral_pmf_of_set)
-          subgoal by(simp add: measure_pmf_of_set)
-          done
+      fix h :: "'a \<Rightarrow> 'b option"    
+
+      fix \<rho>::real
+      assume "\<rho>>0"
+  let ?bl' = "(\<lambda>v h i. if i<m then v * ( (case (S' i) of (x,y) \<Rightarrow> if h x \<noteq> Some y then 1::real else 0)  
+                         -  (case (S i) of (x,y) \<Rightarrow> if h x \<noteq> Some y then 1::real else 0))
+                        else 1)"
+      have "measure_pmf.prob (Samples1 m (pmf_of_set {-1,1::real})) {\<sigma>. \<bar>?bla \<sigma> h\<bar> > \<rho> }
+                   = measure_pmf.prob (Pi_pmf {0..<m} 1 (\<lambda>_. pmf_of_set {- 1, 1}))
+          {\<sigma>. \<rho> < \<bar>(\<Sum>i = 0..<m. ?bl (\<sigma> i) h i) / real m\<bar>}" unfolding Samples1_def by simp
+      also have "\<dots> = measure_pmf.prob 
+            (map_pmf (\<lambda>\<sigma>. (\<lambda>i. ?bl' (\<sigma> i) h i)) (Pi_pmf {0..<m} 1 (\<lambda>_. pmf_of_set {- 1, 1})))
+                  {\<sigma>. \<rho> < \<bar>(\<Sum>i = 0..<m. \<sigma> i) / real m\<bar>}"
+        apply simp done
+      also have "\<dots> = measure_pmf.prob (Pi_pmf {0..<m} 1 
+              (\<lambda>i. map_pmf (\<lambda>v. ?bl' v h i) (pmf_of_set {- 1, 1})))
+          {\<sigma>. \<rho> < \<bar>(\<Sum>i = 0..<m. \<sigma> i) / real m\<bar>}"
+        apply (subst Pi_pmf_map2[where dflt=1]) apply simp apply simp apply simp done 
+      also have "\<dots> = measure_pmf.prob (Pi_pmf {0..<m} 1 
+              (\<lambda>i. map_pmf (\<lambda>v. ?bl' v h i) (pmf_of_set {- 1, 1})))
+          {\<sigma>. \<rho> < \<bar>(\<Sum>i = 0..<m. \<sigma> i)\<bar> / real m}"
+        apply(rule arg_cong[where f="measure_pmf.prob (Pi_pmf {0..<m} 1 
+              (\<lambda>i. map_pmf (\<lambda>v. ?bl' v h i) (pmf_of_set {- 1, 1})))"])
+        by auto
+      also have "\<dots>   \<le> 2 * exp (-  real m  * \<rho>^2 / 2)"
+        apply(rule order.trans) 
+         apply(rule hoeffding_ineq_forreal[where \<mu>="\<lambda>i.0" and a="-1" and b="1", simplified])
+        subgoal by (simp add: integral_pmf_of_set)  
+        subgoal for i apply (simp add: measure_pmf_of_set)
+          apply(cases "S i"; cases "S' i") by auto
+        subgoal apply fact done
+        subgoal by simp
         done
+      finally have "measure_pmf.prob (Samples1 m (pmf_of_set {-1,1::real})) {\<sigma>. \<bar>?bla \<sigma> h\<bar> > \<rho> }
+                \<le> 2 * exp (-  real m  * \<rho>^2 / 2)" .
+   
     } note gaga = this
+ 
 
     have argh: "\<And>\<rho>. {\<sigma>. MAXIMUM (restrictH H_map ?C Y) (\<lambda>h. \<bar>?bla \<sigma> h\<bar>) > \<rho> }
                   \<subseteq> (\<Union>h\<in>(restrictH H_map ?C Y).  {\<sigma>. \<bar>?bla \<sigma> h\<bar> > \<rho>} )"
@@ -532,7 +1159,7 @@ proof -
       thm measure_pmf.finite_measure_subadditive_finite
 
       {fix \<rho> :: real
-
+        assume rhogt0: "\<rho>>0" 
         have "measure_pmf.prob (Samples1 m (pmf_of_set {-1,1::real})) {\<sigma>. MAXIMUM (restrictH H_map ?C Y) (\<lambda>h. \<bar>?bla \<sigma> h\<bar>) > \<rho> }
           \<le> measure_pmf.prob (Samples1 m (pmf_of_set {-1,1::real})) (\<Union>h\<in>(restrictH H_map ?C Y).  {\<sigma>. \<bar>?bla \<sigma> h\<bar> > \<rho>} )"
           apply(rule subsetlesspmf) by(rule argh)
@@ -543,7 +1170,7 @@ proof -
           subgoal by auto
           done
         also have "\<dots> \<le> (\<Sum>h\<in>restrictH H_map ?C Y. 2 * exp (-  real m  * \<rho>^2 / 2) )" 
-           apply(rule sum_mono) by (rule gaga)
+           apply(rule sum_mono) apply (rule gaga) using rhogt0 by simp
         also have "\<dots> = 2 * card (restrictH H_map ?C Y) * exp (-  m  * \<rho>^2 / 2)" 
           apply(subst sum_constant_scale) by simp
         finally
@@ -571,7 +1198,7 @@ proof -
                                             and f="\<lambda>\<sigma>. MAXIMUM (restrictH H_map ?C Y) (\<lambda>h. \<bar>?bla \<sigma> h\<bar> )"  ]
     have therule: "\<And>R. 0 < 1 / sqrt (real m / 2) \<Longrightarrow>
 exp 1 \<le> real (card (restrictH H_map ?C Y)) \<Longrightarrow>
-(\<And>t. 0 \<le> t \<Longrightarrow>
+(\<And>t. 0 < t \<Longrightarrow>
       measure_pmf.prob R
        {x. t < \<bar>(MAX h\<in>restrictH H_map ({fst (S i) |i. i \<in> {0..<m}} \<union> {fst (S' i) |i. i \<in> {0..<m}}) Y.
                     \<bar>?bla x h\<bar>) -
@@ -614,7 +1241,7 @@ measure_pmf.expectation R
         apply(rule order.trans) apply(subst pap)
         subgoal using finite_restrC by simp
         subgoal using restrictH_nonempty by simp
-         apply(rule ppp[of t]) apply simp
+         apply(rule ppp[of t]) apply simp apply simp
         apply(rule mult_left_mono)
         subgoal using m_gt0 by (auto simp: power_divide)     
         subgoal by simp
@@ -652,6 +1279,8 @@ measure_pmf.expectation R
            (\<lambda>S. \<Squnion>h\<in>H. \<bar>measure_pmf.expectation (Samples m D) (\<lambda>S'. TrainErr S' {0..<m} h - TrainErr S {0..<m} h )
                \<bar>)"
     apply(rule expectation_mono)
+    subgoal sorry
+    subgoal sorry
     apply(rule cSUP_mono[OF nnH])
     subgoal sorry
     subgoal for x n apply(rule bexI[where x=n]) sorry (* not sure here! *)
@@ -660,6 +1289,8 @@ measure_pmf.expectation R
            (\<lambda>S. \<Squnion>h\<in>H. measure_pmf.expectation (Samples m D)
          (\<lambda>S'. \<bar>TrainErr S' {0..<m} h - TrainErr S {0..<m} h\<bar> ) )"
     apply(rule expectation_mono)
+    subgoal sorry
+    subgoal sorry
     apply(rule cSUP_mono[OF nnH])
     subgoal sorry
     subgoal for x n apply(rule bexI[where x=n])
@@ -679,6 +1310,8 @@ measure_pmf.expectation R
            (\<lambda>S.  measure_pmf.expectation (Samples m D)
          (\<lambda>S'. \<Squnion>h\<in>H. \<bar>TrainErr S' {0..<m} h - TrainErr S {0..<m} h\<bar> ) )"
       apply(rule expectation_mono) 
+    subgoal sorry
+    subgoal sorry
       apply(rule expectation_Sup_le) done 
     also have "\<dots> = measure_pmf.expectation (Samples m D)
            (\<lambda>S.  measure_pmf.expectation (Samples m D)
@@ -766,9 +1399,12 @@ measure_pmf.expectation R
            (\<lambda>S.  measure_pmf.expectation (Samples m D)
          (\<lambda>S'. ?bnd * \<delta>))"
       apply(rule expectation_mono)
+      subgoal sorry
+      subgoal sorry
       apply(rule expectation_mono)
-      apply(rule fff)
-      done
+      subgoal sorry
+      subgoal sorry
+      apply(rule fff) by auto 
     also have "\<dots> =   ?bnd * \<delta>"
       apply(subst expectation_const)
       apply(subst expectation_const) ..
